upgrade to Isabelle2016-1 and afp-2016-1
git-svn-id: https://projects.brucker.ch/hol-testgen/svn/HOL-TestGen/trunk/hol-testgen@13259 3260e6d1-4efc-4170-b0a7-36055960796d

src/UML_Types.thy
@@ -117,9 +117,9 @@ text{*
   of a bot and a null element. The construction proceeds by
   abstracting the null (defined by @{text "\<lfloor> \<bottom> \<rfloor>"} on
   @{text "'a option option"}) to a @{text null} element, which may
-  have an arbitrary semantic structure, and an undefinedness element @{text "\<bottom> "}
+  have an arbitrary semantic structure, and an undefinedness element @{text "\<bottom>"}
   to an abstract undefinedness element @{text "bot"} (also written
-  @{text "\<bottom> "} whenever no confusion arises). As a consequence, it is necessary
+  @{text "\<bottom>"} whenever no confusion arises). As a consequence, it is necessary
   to redefine the notions of invalid, defined, valuation etc.
   on top of this interface. *}
 
@@ -388,7 +388,7 @@ text{* The core of an own type construction is done via a type
   interface discussed in the previous section. *}
 
 typedef (overloaded) ('\<alpha>, '\<beta>) Pair\<^sub>b\<^sub>a\<^sub>s\<^sub>e = "{X::('\<alpha>::null \<times> '\<beta>::null) option option.
-                                       X = bot \<or> X = null \<or> (fst\<lceil>\<lceil>X\<rceil>\<rceil> \<noteq> bot \<and> snd\<lceil>\<lceil>X\<rceil>\<rceil> \<noteq> bot)}"
+                                           X = bot \<or> X = null \<or> (fst\<lceil>\<lceil>X\<rceil>\<rceil> \<noteq> bot \<and> snd\<lceil>\<lceil>X\<rceil>\<rceil> \<noteq> bot)}"
                             by (rule_tac x="bot" in exI, simp)
 
 text{* We ``carve'' out from the concrete type @{typ "('\<alpha>::null \<times> '\<beta>::null) option option"} 
@@ -514,7 +514,7 @@ text{* The core of an own type construction is done via a type
   interface discussed in the previous section. *}
 
 typedef (overloaded) '\<alpha> Sequence\<^sub>b\<^sub>a\<^sub>s\<^sub>e ="{X::('\<alpha>::null) list option option.
-                              X = bot \<or> X = null \<or> (\<forall>x\<in>set \<lceil>\<lceil>X\<rceil>\<rceil>. x \<noteq> bot)}"
+                                        X = bot \<or> X = null \<or> (\<forall>x\<in>set \<lceil>\<lceil>X\<rceil>\<rceil>. x \<noteq> bot)}"
           by (rule_tac x="bot" in exI, simp)
 
 instantiation   Sequence\<^sub>b\<^sub>a\<^sub>s\<^sub>e  :: (null)bot
@@ -608,8 +608,8 @@ fun disp_msg title msg status = title ^ ": '" ^ msg ^ "' " ^ status
 fun lemma msg specification_theorem concl in_local thy =
   SOME
     (in_local (fn lthy =>
-           specification_theorem Thm.theoremK NONE (K I) (@{binding ""}, []) [] [] 
-             (Element.Shows [((@{binding ""}, []),[(concl lthy, [])])])
+           specification_theorem Thm.theoremK NONE (K I) Binding.empty_atts [] [] 
+             (Element.Shows [(Binding.empty_atts, [(concl lthy, [])])])
              false lthy
         |> Proof.global_terminal_proof
              ((Method.Combinator ( Method.no_combinator_info
@@ -624,9 +624,9 @@ fun outer_syntax_command command_spec theory in_local =
   Outer_Syntax.command command_spec "assert that the given specification is true"
     (Parse.term >> (fn elems_concl => theory (fn thy =>
       case
-        lemma "code_unfold" Specification.theorem
+        lemma "code_unfold" (Specification.theorem true)
           (fn lthy => 
-            let val expr = Value.value lthy (Syntax.read_term lthy elems_concl)
+            let val expr = Value_Command.value lthy (Syntax.read_term lthy elems_concl)
                 val thy = Proof_Context.theory_of lthy
                 open HOLogic in
             if Sign.typ_equiv thy (fastype_of expr, @{typ "prop"}) then
@@ -637,7 +637,7 @@ fun outer_syntax_command command_spec theory in_local =
           thy
       of  NONE => 
             let val attr_simp = "simp" in
-            case lemma attr_simp Specification.theorem_cmd (K elems_concl) in_local thy of
+            case lemma attr_simp (Specification.theorem_cmd true) (K elems_concl) in_local thy of
                NONE => raise (ERROR "Assertion failed")
              | SOME thy => 
                 (writeln (disp_msg "OK" "simp" "finished the normalization");
@@ -648,13 +648,7 @@ fun outer_syntax_command command_spec theory in_local =
             end
         | SOME thy => thy)))
 
-fun in_local decl thy =
-  thy
-  |> Named_Target.init ""
-  |> decl
-  |> Local_Theory.exit_global
-
-val () = outer_syntax_command @{command_keyword Assert} Toplevel.theory in_local 
+val () = outer_syntax_command @{command_keyword Assert} Toplevel.theory Named_Target.theory_map
 val () = outer_syntax_command @{command_keyword Assert_local} (Toplevel.local_theory NONE NONE) I
 (* TO BE DONE  merge the two commands together *)
 *}
