src/compiler/core/Floor1_infra.thy
@@ -69,7 +69,7 @@ definition "print_infra_datatype_class_1 = start_map'' O.datatype o (\<lambda>ex
         (isub_name datatype_name)
         [ (isub_name datatype_constr_name, Raw (isub_name datatype_ext_name) # map_ty l_attr ) ] ]) expr)"
 
-definition' \<open>print_latex_infra_datatype_class = start_map'' O.datatype o (\<lambda>expr _ base_attr' _. map_class_gen_h''''
+definition \<open>print_latex_infra_datatype_class = start_map'' O.datatype o (\<lambda>expr _ base_attr' _. map_class_gen_h''''
   (\<lambda>isub_name name _ l_attr l_inherited l_cons.
     let (l_attr, l_inherited) = base_attr' (l_attr, of_inh l_inherited)
       ; map_ty = L.map ((\<lambda>x. Typ_apply (Typ_base \<open>option\<close>) [str_hol_of_ty_all Typ_apply Typ_base x]) o snd)
